src/DY.Core.Trace.Invariant.fst
@@ -7,32 +7,31 @@ open DY.Core.Label.Type
 open DY.Core.Label
 
 noeq
-type trace_predicates (cpreds:crypto_predicates) = {
-  state_pred: trace -> principal -> nat -> bytes -> prop;
-  state_pred_later:
+type state_predicate (cpreds:crypto_predicates) = {
+  pred: trace -> principal -> nat -> bytes -> prop;
+  // TODO: Do we want the later lemma?
+  pred_later:
     tr1:trace -> tr2:trace ->
     prin:principal -> sess_id:nat -> content:bytes ->
     Lemma
-    (requires state_pred tr1 prin sess_id content /\ tr1 <$ tr2)
-    (ensures state_pred tr2 prin sess_id content)
+    (requires pred tr1 prin sess_id content /\ tr1 <$ tr2)
+    (ensures pred tr2 prin sess_id content)
   ;
-  state_pred_knowable:
+  pred_knowable:
     tr:trace ->
     prin:principal -> sess_id:nat -> content:bytes ->
     Lemma
-    (requires state_pred tr prin sess_id content)
+    (requires pred tr prin sess_id content)
     (ensures
       is_knowable_by cpreds (principal_state_label prin sess_id) tr content
     )
   ;
+}
 
+noeq
+type trace_predicates (cpreds:crypto_predicates) = {
+  state_pred: state_predicate cpreds;
   event_pred: trace -> principal -> string -> bytes -> prop;
-  event_pred_later:
-    tr1:trace -> tr2:trace ->
-    prin:principal -> tag:string -> content:bytes ->
-    Lemma
-    (requires event_pred tr1 prin tag content /\ tr1 <$ tr2)
-    (ensures event_pred tr2 prin tag content)
 }
 
 noeq
@@ -51,7 +50,7 @@ let rec trace_invariant preds tr =
       | MsgSent msg ->
         is_publishable preds.crypto_preds tr msg
       | SetState prin sess_id content -> (
-        preds.trace_preds.state_pred tr_init prin sess_id content
+        preds.trace_preds.state_pred.pred tr_init prin sess_id content
       )
       | Event prin tag content -> (
         preds.trace_preds.event_pred tr_init prin tag content
@@ -62,6 +61,7 @@ let rec trace_invariant preds tr =
 // TODO: the next lemmas have similar proofs
 // maybe refactor?
 
+// Lemma for attacker theorem
 val msg_sent_on_network_are_publishable:
   preds:protocol_predicates -> tr:trace -> msg:bytes ->
   Lemma
@@ -84,6 +84,37 @@ let rec msg_sent_on_network_are_publishable preds tr msg =
     assert(tr_init <$ tr);
     msg_sent_on_network_are_publishable preds tr_init msg
 
+
+val state_was_set_implies_pred:
+  preds:protocol_predicates -> tr:trace ->
+  prin:principal -> sess_id:nat -> content:bytes ->
+  Lemma
+  (requires
+    trace_invariant preds tr /\
+    state_was_set tr prin sess_id content
+  )
+  (ensures preds.trace_preds.state_pred.pred tr prin sess_id content)
+  [SMTPat (state_was_set tr prin sess_id content);
+   SMTPat (trace_invariant preds tr);
+  ]
+let rec state_was_set_implies_pred preds tr prin sess_id content =
+  match tr with
+  | Nil -> assert(False)
+  | Snoc tr_init (SetState prin' sess_id' content') -> (
+    assert(tr_init <$ tr);
+    if prin = prin' && sess_id = sess_id' && content = content' then (
+      preds.trace_preds.state_pred.pred_later tr_init tr prin sess_id content
+    ) else (
+      state_was_set_implies_pred preds tr_init prin sess_id content;
+      preds.trace_preds.state_pred.pred_later tr_init tr prin sess_id content
+    )
+  )
+  | Snoc tr_init _ ->
+    assert(tr_init <$ tr);
+    state_was_set_implies_pred preds tr_init prin sess_id content;
+    preds.trace_preds.state_pred.pred_later tr_init tr prin sess_id content
+
+// Lemma for attacker theorem
 val state_is_knowable_by:
   preds:protocol_predicates -> tr:trace ->
   prin:principal -> sess_id:nat -> content:bytes ->
@@ -93,42 +124,24 @@ val state_is_knowable_by:
     state_was_set tr prin sess_id content
   )
   (ensures is_knowable_by preds.crypto_preds (principal_state_label prin sess_id) tr content)
-let rec state_is_knowable_by preds tr prin sess_id content =
-  match tr with
-  | Nil -> assert(False)
-  | Snoc tr_init (SetState prin' sess_id' content') -> (
-    assert(tr_init <$ tr);
-    if prin = prin' && sess_id = sess_id' && content = content' then (
-      preds.trace_preds.state_pred_knowable tr_init prin sess_id content
-    ) else (
-      state_is_knowable_by preds tr_init prin sess_id content
-    )
-  )
-  | Snoc tr_init _ ->
-    assert(tr_init <$ tr);
-    state_is_knowable_by preds tr_init prin sess_id content
+let state_is_knowable_by preds tr prin sess_id content =
+  preds.trace_preds.state_pred.pred_knowable tr prin sess_id content
 
-// TODO: Does this lemma fits here?
-val event_triggered_implies_pred:
+val event_triggered_at_implies_pred:
   preds:protocol_predicates -> tr:trace ->
-  prin:principal -> tag:string -> content:bytes ->
+  i:nat -> prin:principal -> tag:string -> content:bytes ->
   Lemma
   (requires
-    event_triggered tr prin tag content /\
+    event_triggered_at tr i prin tag content /\
     trace_invariant preds tr
   )
-  (ensures preds.trace_preds.event_pred tr prin tag content)
-let rec event_triggered_implies_pred preds tr prin tag content =
-  match tr with
-  | Nil -> assert(False)
-  | Snoc tr_init (Event prin' tag' content') -> (
-    if prin = prin' && tag = tag' && content = content' then (
-      preds.trace_preds.event_pred_later tr_init tr prin tag content
-    ) else (
-      event_triggered_implies_pred preds tr_init prin tag content;
-      preds.trace_preds.event_pred_later tr_init tr prin tag content
-    )
+  (ensures preds.trace_preds.event_pred (prefix tr i) prin tag content)
+  [SMTPat (event_triggered_at tr i prin tag content);
+   SMTPat (trace_invariant preds tr);
+  ]
+let rec event_triggered_at_implies_pred preds tr i prin tag content =
+  if i+1 = DY.Core.Trace.Type.length tr then ()
+  else (
+    let Snoc tr_init _ = tr in
+    event_triggered_at_implies_pred preds tr_init i prin tag content
   )
-  | Snoc tr_init _ ->
-    event_triggered_implies_pred preds tr_init prin tag content;
-    preds.trace_preds.event_pred_later tr_init tr prin tag content
