src/DY.Core.Trace.Type.fst
@@ -5,7 +5,7 @@ open DY.Core.Label.Type
 
 type trace_event =
   | MsgSent: bytes -> trace_event
-  | RandGen: trace_event
+  | RandGen: lab:label -> len:nat{len <> 0} -> trace_event
   | Corrupt: prin:principal -> sess_id:nat -> trace_event
   | SetState: prin:principal -> sess_id:nat -> content:bytes -> trace_event
   | Event: prin:principal -> tag:string -> content:bytes -> trace_event
@@ -20,13 +20,18 @@ let rec length tr =
   | Nil -> 0
   | Snoc init last -> length init + 1
 
-val grows: trace -> trace -> prop
-let rec grows tr1 tr2 =
-  if length tr1 >= length tr2 then
-    tr1 == tr2
+val prefix: tr:trace -> i:nat{i <= length tr} -> trace
+let rec prefix tr i =
+  if length tr = i then
+    tr
   else
-    let Snoc tr2_init _ = tr2 in
-    grows tr1 tr2_init
+    let Snoc tr_init _ = tr in
+    prefix tr_init i
+
+val grows: trace -> trace -> prop
+let grows tr1 tr2 =
+  length tr1 <= length tr2 /\
+  tr1 == prefix tr2 (length tr1)
 
 let (<$) = grows
 
@@ -44,6 +49,26 @@ let rec grows_transitive tr1 tr2 tr3 =
     grows_transitive tr1 tr2 tr3_init
   )
 
+val length_prefix:
+  tr:trace -> i:nat{i <= length tr} ->
+  Lemma
+  (ensures length (prefix tr i) == i)
+  [SMTPat (length (prefix tr i))]
+let rec length_prefix tr i =
+  if length tr = i then ()
+  else
+    let Snoc tr_init _ = tr in
+    length_prefix tr_init i
+
+val prefix_grows:
+  tr:trace -> i:nat{i <= length tr} ->
+  Lemma
+  (ensures (prefix tr i) <$ tr)
+  //TODO: is this SMTPat dangerous? Should we restrict it to the "safe" on below?
+  [SMTPat (prefix tr i)]
+  //[SMTPat ((prefix tr i) <$ tr)]
+let prefix_grows tr i = ()
+
 //type stable_trace_pred =
 //  pred:(trace -> prop){forall tr1 tr2. tr1 <$ tr2 /\ pred tr1 ==> pred tr2}
 //
@@ -59,25 +84,26 @@ let rec grows_transitive tr1 tr2 tr3 =
 //  );
 //  pred
 
-val event_at: trace -> trace_event -> nat -> prop
-let rec event_at tr e i =
-  if i >= length tr then
-    False
-  else if i+1 = length tr then
+val get_event_at: tr:trace -> i:nat{i < length tr} -> trace_event
+let rec get_event_at tr i =
+  if i+1 = length tr then
     let Snoc _ last = tr in
-    e == last
+    last
   else (
-    assert(i < length tr); // Sanity check
-    let Snoc init _ = tr in
-    event_at init e i
+    let Snoc tr_init _ = tr in
+    get_event_at tr_init i
   )
 
+val event_at: trace -> nat -> trace_event -> prop
+let event_at tr i e =
+  if i >= length tr then
+    False
+  else
+    e == get_event_at tr i
+
 val event_exists: trace -> trace_event -> prop
-let rec event_exists tr e =
-  match tr with
-  | Nil -> False
-  | Snoc tr_init event_last ->
-    event_exists tr_init e \/ e == event_last
+let event_exists tr e =
+  exists i. event_at tr i e
 
 val length_grows:
   tr1:trace -> tr2:trace ->
@@ -94,33 +120,18 @@ let rec length_grows tr1 tr2 =
 
 val event_at_grows:
   tr1:trace -> tr2:trace ->
-  e:trace_event -> i:nat ->
+  i:nat -> e:trace_event ->
   Lemma
-  (requires event_at tr1 e i /\ tr1 <$ tr2)
-  (ensures event_at tr2 e i)
-  [SMTPat (event_at tr1 e i); SMTPat (tr1 <$ tr2)]
-let rec event_at_grows tr1 tr2 e i =
+  (requires event_at tr1 i e /\ tr1 <$ tr2)
+  (ensures event_at tr2 i e)
+  [SMTPat (event_at tr1 i e); SMTPat (tr1 <$ tr2)]
+let rec event_at_grows tr1 tr2 i e =
   if i >= length tr1 then ()
   else if length tr1 >= length tr2 then ()
   else (
     let Snoc tr2_init _ = tr2 in
-    event_at_grows tr1 tr2_init e i
+    event_at_grows tr1 tr2_init i e
   )
-
-val event_exists_grows:
-  tr1:trace -> tr2:trace ->
-  e:trace_event ->
-  Lemma
-  (requires event_exists tr1 e /\ tr1 <$ tr2)
-  (ensures event_exists tr2 e)
-  [SMTPat (event_exists tr1 e); SMTPat (tr1 <$ tr2)]
-let rec event_exists_grows tr1 tr2 e =
-  if length tr1 >= length tr2 then ()
-  else
-    let Snoc tr2_init _ = tr2 in
-    event_exists_grows tr1 tr2_init e
-
-
 
 val msg_sent_on_network: trace -> bytes -> prop
 let msg_sent_on_network tr msg =
@@ -134,6 +145,17 @@ val was_corrupt: trace -> principal -> nat -> prop
 let was_corrupt tr prin sess_id =
   event_exists tr (Corrupt prin sess_id)
 
+val event_triggered_at: trace -> nat -> principal -> string -> bytes -> prop
+let event_triggered_at tr i prin tag content =
+  event_at tr i (Event prin tag content)
+
 val event_triggered: trace -> principal -> string -> bytes -> prop
 let event_triggered tr prin tag content =
-  event_exists tr (Event prin tag content)
+  exists i. event_triggered_at tr i prin tag content
+
+val rand_generated_at: trace -> nat -> bytes -> prop
+let rand_generated_at tr i b =
+  match b with
+  | Rand lab len time ->
+    time == i /\ event_at tr i (RandGen lab len)
+  | _ -> False
