src/DY.Lib.State.Typed.fst
@@ -50,20 +50,27 @@ val has_typed_session_pred:
   #a:Type -> {|parseable_serializeable bytes a|} ->
   preds:protocol_predicates -> string -> typed_session_pred a ->
   prop
-let has_typed_session_pred #a preds lab spred =
-  has_session_pred preds lab (typed_session_pred_to_session_pred spred)
+let has_typed_session_pred #a #ps_a preds label spred =
+  has_session_pred preds label (typed_session_pred_to_session_pred spred)
+
+val typed_state_was_set:
+  #a:Type -> {|parseable_serializeable bytes a|} ->
+  trace -> string -> principal -> nat -> a ->
+  prop
+let typed_state_was_set #a #ps_a tr label prin sess_id content =
+  labeled_state_was_set tr label prin sess_id (serialize _ content)
 
 val set_typed_state:
   #a:Type -> {|parseable_serializeable bytes a|} ->
   string -> principal -> nat -> a -> crypto unit
-let set_typed_state lab prin sess_id content =
-  set_labeled_state lab prin sess_id (serialize _ content)
+let set_typed_state label prin sess_id content =
+  set_labeled_state label prin sess_id (serialize _ content)
 
 val get_typed_state:
   #a:Type -> {|parseable_serializeable bytes a|} ->
   string -> principal -> nat -> crypto (option a)
-let get_typed_state #a lab prin sess_id =
-  let*? content_bytes = get_labeled_state lab prin sess_id in
+let get_typed_state #a label prin sess_id =
+  let*? content_bytes = get_labeled_state label prin sess_id in
   match parse a content_bytes with
   | None -> return None
   | Some content -> return (Some content)
@@ -81,12 +88,13 @@ val set_typed_state_invariant:
   )
   (ensures (
     let ((), tr_out) = set_typed_state label prin sess_id content tr in
-    trace_invariant preds tr_out
+    trace_invariant preds tr_out /\
+    typed_state_was_set tr_out label prin sess_id content
   ))
   [SMTPat (set_typed_state label prin sess_id content tr);
    SMTPat (trace_invariant preds tr);
    SMTPat (has_typed_session_pred preds label spred)]
-let set_typed_state_invariant #a #ps_a preds lab spred prin sess_id content tr =
+let set_typed_state_invariant #a #ps_a preds label spred prin sess_id content tr =
   parse_serialize_inv_lemma #bytes a content
 
 val get_typed_state_invariant:
@@ -112,4 +120,24 @@ val get_typed_state_invariant:
   [SMTPat (get_typed_state #a label prin sess_id tr);
    SMTPat (trace_invariant preds tr);
    SMTPat (has_typed_session_pred preds label spred)]
-let get_typed_state_invariant #a #ps_a preds lab spred prin sess_id tr = ()
+let get_typed_state_invariant #a #ps_a preds label spred prin sess_id tr = ()
+
+val typed_state_was_set_implies_pred:
+  #a:Type -> {|parseable_serializeable bytes a|} ->
+  preds:protocol_predicates -> tr:trace ->
+  label:string -> spred:typed_session_pred a ->
+  prin:principal -> sess_id:nat -> content:a ->
+  Lemma
+  (requires
+    typed_state_was_set tr label prin sess_id content /\
+    trace_invariant preds tr /\
+    has_typed_session_pred preds label spred
+  )
+  (ensures spred.pred preds.crypto_preds tr prin sess_id content)
+  [SMTPat (typed_state_was_set tr label prin sess_id content);
+   SMTPat (trace_invariant preds tr);
+   SMTPat (has_typed_session_pred preds label spred);
+  ]
+let typed_state_was_set_implies_pred #a #ps_a preds tr label spred prin sess_id content =
+  parse_serialize_inv_lemma #bytes a content;
+  ()
