src/DY.Example.NSL.Protocol.Stateful.fst
@@ -1,0 +1,131 @@
+module DY.Example.NSL.Protocol.Stateful
+
+open Comparse
+open DY.Core
+open DY.Lib
+open DY.Example.NSL.Protocol.Total
+
+type nsl_session_ (bytes:Type0) {|bytes_like bytes|} =
+  | InitiatorSentMsg1: b:principal -> n_a:bytes -> nsl_session_ bytes
+  | ResponderSentMsg2: a:principal -> n_a:bytes -> n_b:bytes -> nsl_session_ bytes
+  | InitiatorSentMsg3: b:principal -> n_a:bytes -> n_b:bytes -> nsl_session_ bytes
+  | ResponderReceivedMsg3: a:principal -> n_a:bytes -> n_b:bytes -> nsl_session_ bytes
+
+%splice [ps_nsl_session_] (gen_parser (`nsl_session_))
+%splice [ps_nsl_session__is_well_formed] (gen_is_well_formed_lemma (`nsl_session_))
+
+type nsl_session = nsl_session_ bytes
+
+instance nsl_session_parseable_serializeable (bytes:Type0) {|bytes_like bytes|}: parseable_serializeable bytes (nsl_session_ bytes)
+ = mk_parseable_serializeable ps_nsl_session_
+
+val nsl_session_label: string
+let nsl_session_label = "NSL.Session"
+
+type nsl_event_ (bytes:Type0) {|bytes_like bytes|} =
+  | Initiate1: a:principal -> b:principal -> n_a:bytes -> nsl_event_ bytes
+  | Respond1: a:principal -> b:principal -> n_a:bytes -> n_b:bytes -> nsl_event_ bytes
+  | Initiate2: a:principal -> b:principal -> n_a:bytes -> n_b:bytes -> nsl_event_ bytes
+  | Respond2: a:principal -> b:principal -> n_a:bytes -> n_b:bytes -> nsl_event_ bytes
+
+%splice [ps_nsl_event_] (gen_parser (`nsl_event_))
+%splice [ps_nsl_event__is_well_formed] (gen_is_well_formed_lemma (`nsl_event_))
+
+type nsl_event = nsl_event_ bytes
+
+instance nsl_event_parseable_serializeable (bytes:Type0) {|bytes_like bytes|}: parseable_serializeable bytes (nsl_event_ bytes)
+ = mk_parseable_serializeable ps_nsl_event_
+
+val nsl_event_label: string
+let nsl_event_label = "NSL.Event"
+
+type nsl_global_sess_ids = {
+  pki: nat;
+  private_keys: nat;
+}
+
+val prepare_msg1: principal -> principal -> crypto nat
+let prepare_msg1 alice bob =
+  let* n_a = mk_rand (join (principal_label alice) (principal_label bob)) 32 in
+  trigger_event alice nsl_event_label (serialize nsl_event (Initiate1 alice bob n_a));*
+  let* sess_id = new_session_id alice in
+  set_typed_state nsl_session_label alice sess_id (InitiatorSentMsg1 bob n_a <: nsl_session);*
+  return sess_id
+
+val send_msg1: nsl_global_sess_ids -> principal -> nat -> crypto (option nat)
+let send_msg1 global_sess_id alice sess_id =
+  let*? st: nsl_session = get_typed_state nsl_session_label alice sess_id in
+  match st with
+  | InitiatorSentMsg1 bob n_a -> (
+    let*? pk_b = get_public_key alice global_sess_id.pki PkEnc bob in
+    let* nonce = mk_rand (principal_label alice) 32 in
+    let msg = compute_message1 alice bob pk_b n_a nonce in
+    let* msg_id = send_msg msg in
+    return (Some msg_id)
+  )
+  | _ -> return None
+
+val prepare_msg2: nsl_global_sess_ids -> principal -> nat -> crypto (option nat)
+let prepare_msg2 global_sess_id bob msg_id =
+  let*? msg = recv_msg msg_id in
+  let*? sk_b = get_private_key bob global_sess_id.private_keys PkDec in
+  let*? msg1: message1 = return (decode_message1 bob msg sk_b) in
+  let* n_b = mk_rand (join (principal_label msg1.alice) (principal_label bob)) 32 in
+  trigger_event bob nsl_event_label (serialize nsl_event (Respond1 msg1.alice bob msg1.n_a n_b));*
+  let* sess_id = new_session_id bob in
+  set_typed_state nsl_session_label bob sess_id (ResponderSentMsg2 msg1.alice msg1.n_a n_b <: nsl_session);*
+  return (Some sess_id)
+
+val send_msg2: nsl_global_sess_ids -> principal -> nat -> crypto (option nat)
+let send_msg2 global_sess_id bob sess_id =
+  let*? st: nsl_session = get_typed_state nsl_session_label bob sess_id in
+  match st with
+  | ResponderSentMsg2 alice n_a n_b -> (
+    let*? pk_a = get_public_key bob global_sess_id.pki PkEnc alice in
+    let* nonce = mk_rand (principal_label bob) 32 in
+    let msg = compute_message2 bob {n_a; alice;} pk_a n_b nonce in
+    let* msg_id = send_msg msg in
+    return (Some msg_id)
+  )
+  | _ -> return None
+
+val prepare_msg3: nsl_global_sess_ids -> principal -> nat -> nat -> crypto (option unit)
+let prepare_msg3 global_sess_id alice sess_id msg_id =
+  let*? msg = recv_msg msg_id in
+  let*? sk_a = get_private_key alice global_sess_id.private_keys PkDec in
+  let*? st: nsl_session = get_typed_state nsl_session_label alice sess_id in
+  match st with
+  | InitiatorSentMsg1 bob n_a -> (
+    let*? msg2: message2 = return (decode_message2 alice bob msg sk_a n_a) in
+    trigger_event alice nsl_event_label (serialize nsl_event (Initiate2 alice bob n_a msg2.n_b));*
+    set_typed_state nsl_session_label alice sess_id (InitiatorSentMsg3 bob n_a msg2.n_b <: nsl_session);*
+    return (Some ())
+  )
+  | _ -> return None
+
+val send_msg3: nsl_global_sess_ids -> principal -> nat -> crypto (option nat)
+let send_msg3 global_sess_id alice sess_id =
+  let*? st: nsl_session = get_typed_state nsl_session_label alice sess_id in
+  match st with
+  | InitiatorSentMsg3 bob n_a n_b -> (
+    let*? pk_b = get_public_key alice global_sess_id.pki PkEnc bob in
+    let* nonce = mk_rand (principal_label alice) 32 in
+    let msg = compute_message3 alice bob pk_b n_b nonce in
+    let* msg_id = send_msg msg in
+    return (Some msg_id)
+  )
+  | _ -> return None
+
+val prepare_msg4: nsl_global_sess_ids -> principal -> nat -> nat -> crypto (option unit)
+let prepare_msg4 global_sess_id bob sess_id msg_id =
+  let*? msg = recv_msg msg_id in
+  let*? sk_b = get_private_key bob global_sess_id.private_keys PkDec in
+  let*? st: nsl_session = get_typed_state nsl_session_label bob sess_id in
+  match st with
+  | ResponderSentMsg2 alice n_a n_b -> (
+    let*? msg3: message3 = return (decode_message3 alice bob msg sk_b n_b) in
+    trigger_event bob nsl_event_label (serialize nsl_event (Respond2 alice bob n_a n_b));*
+    set_typed_state nsl_session_label bob sess_id (ResponderReceivedMsg3 alice n_a n_b <: nsl_session);*
+    return (Some ())
+  )
+  | _ -> return None
