src/DY.Example.NSL.Protocol.Total.fst
@@ -1,0 +1,117 @@
+module DY.Example.NSL.Protocol.Total
+
+open Comparse
+open DY.Core
+open DY.Lib
+
+// Needham-Schroeder-Lowe Fixed Public Key Protocol [2]
+//
+// A -> B: {N_A, A}K_PB       msg 1
+// B -> A: {N_A, N_B, B}K_PA  msg 2 -- note addition of B
+// A -> B: {N_B}K_PB          msg 3
+//
+// [2] Gavin Lowe. "Breaking and fixing the Needham-Schroeder Public-Key
+//     Protocol using FDR". TACAS, pp 147-166, 1996.
+//
+// Note: the version implemented in DY* has a modified msg 3:
+// it is {N_B, A}K_PB
+
+val (let?): #a:Type -> #b:Type -> x:option a -> (y:a -> Pure (option b) (requires x == Some y) (ensures fun _ -> True)) -> option b
+let (let?) #a #b x f =
+  match x with
+  | None -> None
+  | Some x -> f x
+
+val guard: b:bool -> option unit
+let guard b =
+  if b then Some ()
+  else None
+
+(*** Message 1 ***)
+
+type message1_ (bytes:Type0) {|bytes_like bytes|} = {
+  n_a: bytes;
+  alice: principal;
+}
+
+%splice [ps_message1_] (gen_parser (`message1_))
+%splice [ps_message1__is_well_formed] (gen_is_well_formed_lemma (`message1_))
+
+type message2_ (bytes:Type0) {|bytes_like bytes|} = {
+  n_a: bytes;
+  n_b: bytes;
+  bob: principal;
+}
+
+%splice [ps_message2_] (gen_parser (`message2_))
+%splice [ps_message2__is_well_formed] (gen_is_well_formed_lemma (`message2_))
+
+type message3_ (bytes:Type0) {|bytes_like bytes|} = {
+  n_b: bytes;
+  // The `alice` principal is an addition of DY* example
+  alice: principal;
+}
+
+%splice [ps_message3_] (gen_parser (`message3_))
+%splice [ps_message3__is_well_formed] (gen_is_well_formed_lemma (`message3_))
+
+type message_ (bytes:Type0) {|bytes_like bytes|} =
+  | Msg1: message1_ bytes -> message_ bytes
+  | Msg2: message2_ bytes -> message_ bytes
+  | Msg3: message3_ bytes -> message_ bytes
+
+%splice [ps_message_] (gen_parser (`message_))
+%splice [ps_message__is_well_formed] (gen_is_well_formed_lemma (`message_))
+
+instance parseable_serializeable_message_ (bytes:Type0) {|bytes_like bytes|}: parseable_serializeable bytes (message_ bytes) = mk_parseable_serializeable (ps_message_)
+
+type message = message_ bytes
+type message1 = message1_ bytes
+type message2 = message2_ bytes
+type message3 = message3_ bytes
+
+val compute_message1: principal -> principal -> bytes -> bytes -> bytes -> bytes
+let compute_message1 alice bob pk_b n_a nonce =
+  let msg = Msg1 {n_a; alice;} in
+  pk_enc pk_b nonce (serialize message msg)
+
+val decode_message1: principal -> bytes -> bytes -> option message1
+let decode_message1 bob msg1_cipher sk_b =
+  let? msg1_plain = pk_dec sk_b msg1_cipher in
+  let? msg1 = parse message msg1_plain in
+  guard (Msg1? msg1);?
+  Some (Msg1?._0 msg1)
+
+(*** Message 2 ***)
+
+val compute_message2: principal -> message1 -> bytes -> bytes -> bytes -> bytes
+let compute_message2 bob msg1 pk_a n_b nonce =
+  let msg2 = Msg2 {n_a = msg1.n_a;  n_b; bob;} in
+  pk_enc pk_a nonce (serialize message msg2)
+
+val decode_message2: principal -> principal -> bytes -> bytes -> bytes -> option (message2)
+let decode_message2 alice bob msg2_cipher sk_a n_a =
+  let? msg2_plain = pk_dec sk_a msg2_cipher in
+  let? msg2 = parse _ msg2_plain in
+  guard (Msg2? msg2);?
+  let (Msg2 msg2) = msg2 in
+  guard (n_a = msg2.n_a);?
+  guard (bob = msg2.bob);?
+  Some msg2
+
+(*** Message 3 ***)
+
+val compute_message3: principal -> principal -> bytes -> bytes -> bytes -> bytes
+let compute_message3 alice bob pk_b n_b nonce =
+  let msg3 = Msg3 {n_b; alice;} in
+  pk_enc pk_b nonce (serialize message msg3)
+
+val decode_message3: principal -> principal -> bytes -> bytes -> bytes -> option (message3)
+let decode_message3 alice bob msg_cipher sk_b n_b =
+  let? msg_plain = pk_dec sk_b msg_cipher in
+  let? msg = parse _ msg_plain in
+  guard (Msg3? msg);?
+  let (Msg3 msg3) = msg in
+  guard (n_b = msg3.n_b);?
+  guard (alice = msg3.alice);?
+  Some msg3
