src/DY.Example.NSL.SecurityProperties.fst
@@ -1,0 +1,117 @@
+module DY.Example.NSL.SecurityProperties
+
+open Comparse
+open DY.Core
+open DY.Lib
+open DY.Example.NSL.Protocol.Total.Proof
+open DY.Example.NSL.Protocol.Stateful
+open DY.Example.NSL.Protocol.Stateful.Proof
+
+#set-options "--fuel 0 --ifuel 1 --z3rlimit 25  --z3cliopt 'smt.qi.eager_threshold=100'"
+
+val initiator_authentication:
+  tr:trace -> i:nat ->
+  alice:principal -> bob:principal -> n_a:bytes -> n_b:bytes ->
+  Lemma
+  (requires
+    event_triggered_at tr i bob nsl_event_label (serialize nsl_event (Respond2 alice bob n_a n_b)) /\
+    trace_invariant nsl_protocol_preds tr
+  )
+  (ensures
+    (join (principal_label alice) (principal_label bob)) `can_flow tr` public \/
+    event_triggered (prefix tr i) alice nsl_event_label (serialize nsl_event (Initiate2 alice bob n_a n_b))
+  )
+let initiator_authentication tr i alice bob n_a n_b =
+  parse_serialize_inv_lemma #bytes nsl_event (Respond2 alice bob n_a n_b)
+
+val responder_authentication:
+  tr:trace -> i:nat ->
+  alice:principal -> bob:principal -> n_a:bytes -> n_b:bytes ->
+  Lemma
+  (requires
+    event_triggered_at tr i alice nsl_event_label (serialize nsl_event (Initiate2 alice bob n_a n_b)) /\
+    trace_invariant nsl_protocol_preds tr
+  )
+  (ensures
+    (join (principal_label alice) (principal_label bob)) `can_flow tr` public \/
+    event_triggered (prefix tr i) bob nsl_event_label (serialize nsl_event (Respond1 alice bob n_a n_b))
+  )
+let responder_authentication tr i alice bob n_a n_b =
+  parse_serialize_inv_lemma #bytes nsl_event (Initiate2 alice bob n_a n_b)
+
+val n_a_secrecy:
+  tr:trace -> alice:principal -> bob:principal -> n_a:bytes ->
+  Lemma
+  (requires
+    attacker_knows tr n_a /\
+    trace_invariant nsl_protocol_preds tr /\ (
+      (exists sess_id. typed_state_was_set tr nsl_session_label alice sess_id (InitiatorSentMsg1 bob n_a <: nsl_session)) \/
+      (exists sess_id n_b. typed_state_was_set tr nsl_session_label alice sess_id (InitiatorSentMsg3 bob n_a n_b <: nsl_session)) \/
+      (exists sess_id n_b. typed_state_was_set tr nsl_session_label bob sess_id (ResponderReceivedMsg3 alice n_a n_b <: nsl_session))
+    )
+  )
+  (ensures (join (principal_label alice) (principal_label bob)) `can_flow tr` public)
+let n_a_secrecy tr alice bob n_a =
+  attacker_only_knows_publishable_values nsl_protocol_preds tr n_a;
+  introduce (exists sess_id. typed_state_was_set tr nsl_session_label alice sess_id (InitiatorSentMsg1 bob n_a <: nsl_session)) ==> (join (principal_label alice) (principal_label bob)) `can_flow tr` public with _. (
+    parse_serialize_inv_lemma #bytes nsl_event (Initiate1 alice bob n_a)
+  );
+  introduce (exists sess_id n_b. typed_state_was_set tr nsl_session_label alice sess_id (InitiatorSentMsg3 bob n_a n_b <: nsl_session)) ==> (join (principal_label alice) (principal_label bob)) `can_flow tr` public with _. (
+    eliminate exists sess_id n_b. typed_state_was_set tr nsl_session_label alice sess_id (InitiatorSentMsg3 bob n_a n_b <: nsl_session) returns _ with _. (
+      parse_serialize_inv_lemma #bytes nsl_event (Initiate2 alice bob n_a n_b);
+      parse_serialize_inv_lemma #bytes nsl_event (Initiate1 alice bob n_a);
+      assert(event_triggered tr alice nsl_event_label (serialize nsl_event (Initiate1 alice bob n_a)))
+    )
+  );
+  introduce (exists sess_id n_b. typed_state_was_set tr nsl_session_label bob sess_id (ResponderReceivedMsg3 alice n_a n_b <: nsl_session)) ==> (join (principal_label alice) (principal_label bob)) `can_flow tr` public with _. (
+    eliminate exists sess_id n_b. typed_state_was_set tr nsl_session_label bob sess_id (ResponderReceivedMsg3 alice n_a n_b <: nsl_session) returns _ with _. (
+      parse_serialize_inv_lemma #bytes nsl_event (Respond2 alice bob n_a n_b);
+      parse_serialize_inv_lemma #bytes nsl_event (Initiate2 alice bob n_a n_b);
+      parse_serialize_inv_lemma #bytes nsl_event (Initiate1 alice bob n_a);
+      assert(
+        (join (principal_label alice) (principal_label bob)) `can_flow tr` public \/
+        event_triggered tr alice nsl_event_label (serialize nsl_event (Initiate2 alice bob n_a n_b))
+      );
+      assert(
+        (join (principal_label alice) (principal_label bob)) `can_flow tr` public \/
+        event_triggered tr alice nsl_event_label (serialize nsl_event (Initiate1 alice bob n_a))
+      )
+    )
+  )
+
+val n_b_secrecy:
+  tr:trace -> alice:principal -> bob:principal -> n_b:bytes ->
+  Lemma
+  (requires
+    attacker_knows tr n_b /\
+    trace_invariant nsl_protocol_preds tr /\ (
+      (exists sess_id n_a. typed_state_was_set tr nsl_session_label bob sess_id (ResponderSentMsg2 alice n_a n_b <: nsl_session)) \/
+      (exists sess_id n_a. typed_state_was_set tr nsl_session_label bob sess_id (ResponderReceivedMsg3 alice n_a n_b <: nsl_session)) \/
+      (exists sess_id n_a. typed_state_was_set tr nsl_session_label alice sess_id (InitiatorSentMsg3 bob n_a n_b <: nsl_session))
+    )
+  )
+  (ensures (join (principal_label alice) (principal_label bob)) `can_flow tr` public)
+let n_b_secrecy tr alice bob n_b =
+  attacker_only_knows_publishable_values nsl_protocol_preds tr n_b;
+  introduce (exists sess_id n_a. typed_state_was_set tr nsl_session_label bob sess_id (ResponderSentMsg2 alice n_a n_b <: nsl_session)) ==> (join (principal_label alice) (principal_label bob)) `can_flow tr` public with _. (
+    eliminate exists sess_id n_a. typed_state_was_set tr nsl_session_label bob sess_id (ResponderSentMsg2 alice n_a n_b <: nsl_session) returns _ with _. (
+      parse_serialize_inv_lemma #bytes nsl_event (Respond1 alice bob n_a n_b)
+    )
+  );
+  introduce (exists sess_id n_a. typed_state_was_set tr nsl_session_label bob sess_id (ResponderReceivedMsg3 alice n_a n_b <: nsl_session)) ==> (join (principal_label alice) (principal_label bob)) `can_flow tr` public with _. (
+    eliminate exists sess_id n_a. typed_state_was_set tr nsl_session_label bob sess_id (ResponderReceivedMsg3 alice n_a n_b <: nsl_session) returns _ with _. (
+      parse_serialize_inv_lemma #bytes nsl_event (Respond2 alice bob n_a n_b);
+      parse_serialize_inv_lemma #bytes nsl_event (Respond1 alice bob n_a n_b);
+      assert(event_triggered tr bob nsl_event_label (serialize nsl_event (Respond1 alice bob n_a n_b)))
+    )
+  );
+  introduce (exists sess_id n_a. typed_state_was_set tr nsl_session_label alice sess_id (InitiatorSentMsg3 bob n_a n_b <: nsl_session)) ==> (join (principal_label alice) (principal_label bob)) `can_flow tr` public with _. (
+    eliminate exists sess_id n_a. typed_state_was_set tr nsl_session_label alice sess_id (InitiatorSentMsg3 bob n_a n_b <: nsl_session) returns _ with _. (
+      parse_serialize_inv_lemma #bytes nsl_event (Initiate2 alice bob n_a n_b);
+      parse_serialize_inv_lemma #bytes nsl_event (Respond1 alice bob n_a n_b);
+      assert(
+        (join (principal_label alice) (principal_label bob)) `can_flow tr` public \/
+        event_triggered tr bob nsl_event_label (serialize nsl_event (Respond1 alice bob n_a n_b))
+      )
+    )
+  )
